theories/Decidability/UntypedCompleteness.v
@@ -4,7 +4,7 @@ From Equations Require Import Equations.
 From LogRel Require Import Utils Syntax.All DeclarativeTyping GenericTyping AlgorithmicTyping.
 From LogRel.TypingProperties Require Import DeclarativeProperties PropertiesDefinition SubstConsequences TypeConstructorsInj NeutralConvProperties.
 From LogRel.Algorithmic Require Import BundledAlgorithmicTyping AlgorithmicConvProperties AlgorithmicTypingProperties UntypedAlgorithmicConversion.
-From LogRel.Decidability Require Import Functions UntypedFunctions Soundness UntypedSoundness Completeness.
+From LogRel.Decidability Require Import Functions Views UntypedFunctions Soundness UntypedSoundness Completeness.
 From PartialFun Require Import Monad PartialFun MonadExn.
 
 Set Universe Polymorphism.
