theories/Decidability/UntypedNegativeSoundness.v
@@ -1,0 +1,740 @@
+(** * LogRel.Decidability.UntypedNegativeSoundness: implementation failure implies negation of typing for untyped conversion. *)
+From Coq Require Import Nat Lia Arith.
+From Equations Require Import Equations.
+From LogRel Require Import Utils Syntax.All GenericTyping DeclarativeTyping AlgorithmicTyping.
+From LogRel.TypingProperties Require Import PropertiesDefinition DeclarativeProperties SubstConsequences TypeConstructorsInj NeutralConvProperties.
+From LogRel.Algorithmic Require Import BundledAlgorithmicTyping AlgorithmicConvProperties AlgorithmicTypingProperties.
+From LogRel Require Import UntypedAlgorithmicConversion.
+
+From LogRel.Decidability Require Import Functions UntypedFunctions Views Soundness
+  UntypedSoundness Completeness UntypedCompleteness.
+From PartialFun Require Import Monad PartialFun MonadExn.
+
+Set Universe Polymorphism.
+Set Printing Primitive Projection Parameters.
+Set Structural Injection.
+
+Hint Extern 10 =>
+  match goal with
+    | H : _ × _ |- _ => destruct H
+    | H : ~ _ |- False => apply H
+    | H : [× _, _ & _] |- _ => destruct H 
+    | H : [× _, _, _ & _] |- _ => destruct H 
+    | H : [× _, _, _, _ & _] |- _ => destruct H 
+    | H : [× _, _, _, _, _ & _] |- _ => destruct H 
+    | H : [× _, _, _, _, _, _ & _] |- _ => destruct H 
+    | H : [× _, _, _, _, _, _, _ & _] |- _ => destruct H 
+    | H : [× _, _, _, _, _, _, _, _ & _] |- _ => destruct H 
+    | H : [× _, _, _, _, _, _, _, _, _ & _] |- _ => destruct H
+  end : core.
+
+Import DeclarativeTypingProperties.
+
+Section ConvSoundNeg.
+
+  Context `{!TypingSubst de} `{!TypeConstructorsInj de}
+    `{!TermConstructorsInj de} `{!ConvNeutralConv de}.
+
+  #[universes(polymorphic)]Definition uconv_sound_neg_pre
+    (x : uconv_state × term × term) : Type :=
+  match x with
+  | (tm_state,t,u) => ∑ Γ A, [Γ |- t ∈ A] × [Γ |- u ∈ A]
+  | (tm_red_state,t,u) => ∑ Γ A, [× whnf t, whnf u & ([Γ |- t ∈ A] × [Γ |- u ∈ A])]
+  | (ne_state,m,n) => ∑ Γ, [× whne m, whne n & (well_typed Γ m × well_typed Γ n)]
+  end.
+
+  #[universes(polymorphic)]Definition uconv_sound_neg_type
+    (x : uconv_state × term × term)
+    (r : exn errors unit)
+    (p : uconv_sound_neg_pre x) : Type :=
+  match x, p, r with
+  | _, _, (success _) => True
+  | (tm_state,t,u), (Γ;(A;_)), (exception _) =>  ~ [Γ |-[de] t ≅ u ∈ A]
+  | (tm_red_state,t,u), (Γ;(A;_)), (exception _) => ~ [Γ |-[de] t ≅ u ∈ A]
+  | (ne_state,m,n), (Γ;_), (exception _) => ~ ∑ T, [Γ |-[de] m ~ n : T]
+  end.
+
+  Definition term_class_ty `{ta : tag} `{WfType ta} `{Typing ta} Γ A t :
+    [Γ |-[ta] t : A] -> [Γ |-[ta] t ∈ (isterm A)] :=
+    fun H => H.
+
+  Definition type_class_ty `{ta : tag} `{WfType ta} `{Typing ta} Γ A :
+    [Γ |-[ta] A] -> [Γ |-[ta] A ∈ istype] :=
+    fun H => H.
+
+  Lemma convtm_red' Γ A A' t t' u u' :
+    [t ⤳* t'] ->
+    [u ⤳* u'] ->
+    [A ⤳* A'] ->
+    [Γ |-[de] t ≅ u : A] ->
+    [Γ |-[de] t' ≅ u' : A'].
+  Proof.
+    intros.
+    econstructor.
+    2: eapply subject_reduction_type ; boundary.
+    etransitivity.
+    2: etransitivity ; [eassumption|..].
+    1: symmetry.
+    all: eapply subject_reduction ; tea ; boundary.
+  Qed.
+
+  Lemma pair_conv_fst Γ A A' B B' t t' u u' T :
+    [Γ |-[ de ] tPair A B t u ≅ tPair A' B' t' u' : T] ->
+    [Γ |- t ≅ t' : A].
+  Proof.
+    intros Hty.
+    eapply convtm_red'.
+    3: reflexivity.
+    1-2: eapply redalg_one_step, fstPair.
+    econstructor.
+    eapply convtm_conv ; tea.
+    eapply boundary_tm_conv_l in Hty as (?&[->]&?)%termGen'.
+    now symmetry.
+  Qed.
+
+  Lemma pair_conv_snd Γ A A' B B' t t' u u' T :
+    [Γ |-[ de ] tPair A B t u ≅ tPair A' B' t' u' : T] ->
+    [Γ |- u ≅ u' : B[t..]].
+  Proof.
+    intros Hty.
+    eapply convtm_red'.
+    3: reflexivity.
+    1-2: eapply redalg_one_step, sndPair.
+    econstructor.
+    1: econstructor.
+    1: eapply convtm_conv ; tea.
+    all: eapply boundary_tm_conv_l in Hty as (?&[->]&?)%termGen'.
+    1:  now symmetry.
+    eapply typing_subst1.
+    2: constructor ; boundary.
+    constructor ; boundary.
+  Qed.
+
+  Lemma pair_conv_fst_ne Γ A B t u n' T :
+    [Γ |-[ de ] tPair A B t u ≅ n' : T] ->
+    [Γ |- t ≅ tFst n' : A].
+  Proof.
+    intros Hty.
+    eapply convtm_red'.
+    2,3: reflexivity.
+    1: eapply redalg_one_step, fstPair.
+    econstructor.
+    eapply convtm_conv ; tea.
+    eapply boundary_tm_conv_l in Hty as (?&[->]&?)%termGen'.
+    now symmetry.
+  Qed.
+
+  Lemma pair_conv_snd_ne Γ A B t u n' T :
+    [Γ |-[ de ] tPair A B t u ≅ n' : T] ->
+    [Γ |- u ≅ tSnd n' : B[t..]].
+  Proof.
+    intros Hty.
+    eapply convtm_red'.
+    2,3: reflexivity.
+    1: eapply redalg_one_step, sndPair.
+    econstructor.
+    1: econstructor.
+    1: eapply convtm_conv ; tea.
+    all: eapply boundary_tm_conv_l in Hty as (?&[->]&?)%termGen'.
+    1:  now symmetry.
+    eapply typing_subst1.
+    2: constructor ; boundary.
+    constructor ; boundary.
+  Qed.
+
+Lemma pair_conv_ne_fst Γ n A' B' t' u' T :
+  [Γ |-[ de ] n ≅ tPair A' B' t' u' : T] ->
+  [Γ |- tFst n ≅ t' : A'].
+Proof.
+  intros Hty.
+  eapply convtm_red'.
+  1,3: reflexivity.
+  1: eapply redalg_one_step, fstPair.
+  econstructor.
+  eapply convtm_conv ; tea.
+  eapply boundary_tm_conv_r in Hty as (?&[->]&?)%termGen'.
+  now symmetry.
+Qed.
+
+Lemma pair_conv_ne_snd Γ n A' B' t' u' T :
+  [Γ |-[ de ] n ≅ tPair A' B' t' u' : T] ->
+  [Γ |- tSnd n ≅ u' : B'[t'..]].
+Proof.
+  intros Hty.
+  eapply convtm_red'.
+  1,3: reflexivity.
+  1: eapply redalg_one_step, sndPair.
+  econstructor.
+  1: econstructor.
+  1: eapply convtm_conv ; tea.
+  2: eapply typing_subst1.
+  2: now eapply pair_conv_ne_fst.
+  all: eapply boundary_tm_conv_r in Hty as (?&[->]&?)%termGen'.
+  1: now symmetry.
+  constructor ; boundary.
+Qed.
+
+
+Lemma mismatch2_hd_view_ty Γ T V (tT : isType T) (tV : isType V) :
+  build_nf_view2 T V = mismatch2 T V ->
+  type_hd_view Γ tT tV = False.
+Proof.
+  destruct tT, tV ; cbn ; try reflexivity.
+  all: simp build_nf_view2 ; cbn.
+  1-6: congruence.
+  do 2 (unshelve erewrite whne_nf_view1 ; tea ; cbn).
+  congruence.
+Qed.
+
+Lemma mismatch2_hd_view_tm Γ A t u :
+  [Γ |-[de] t : A] -> [Γ |-[de] u : A] ->
+  whnf t -> whnf u ->
+  build_nf_view2 t u = mismatch2 t u ->
+  (∑ (nft : isType t) (nfu : isType u), type_hd_view Γ nft nfu = False) +
+  ((∑ (nft : isNat t) (nfu : isNat u), nat_hd_view Γ nft nfu = False) +
+  (∑ (nft : isId t) (nfu : isId u) , forall Γ A' x y, id_hd_view Γ A' x y nft nfu = False)).
+Proof.
+  intros Ht Hu wt wu.
+  funelim (build_nf_view2 t u).
+  all: try solve [
+    congruence |
+    match goal with
+      | H : [_ |-[de] (tSort _) : _] |- _ => eapply termGen' in H as (?&[]&?)
+    end |
+    left ; unshelve (do 2 eexists) ; try constructor ; cbn ;
+    now apply not_can_whne ; [..|eapply tm_view1_neutral_can] |
+    right ; left ; unshelve (do 2 eexists) ; try constructor ; cbn ;
+    now apply not_can_whne ; [..|eapply tm_view1_neutral_can]].
+
+    1,4: unshelve (right ; right ; unshelve (do 2 eexists) ; econstructor ;
+      [now apply not_can_whne ; [..|eapply tm_view1_neutral_can]|..] ;
+      do 2 eexists ; reflexivity) ; easy.
+    
+    - destruct t1 ; try solve [congruence |
+      left ; unshelve (do 2 eexists) ; try constructor ; cbn ;
+      now apply not_can_whne ; [..|eapply tm_view1_neutral_can]].
+
+    - destruct n ;
+      try solve [
+      congruence |
+      right ; left ; unshelve (do 2 eexists) ; try constructor ; cbn ;
+      now apply not_can_whne ; [..|eapply tm_view1_neutral_can]].
+
+Qed.
+
+Lemma mismatch2_hd_view_ne t u :
+  whne t -> whne u ->
+  ~ build_nf_view2 t u = mismatch2 t u.
+Proof.
+  intros Ht Hu.
+  funelim (build_nf_view2 _ _) ; try solve [congruence|inversion Hu|inversion Ht].
+  - destruct t1 ; inversion Hu.
+  - destruct n ; inversion Hu.
+Qed. 
+
+  Lemma _implem_uconv_neg_sound :
+    funrect _uconv uconv_sound_neg_pre uconv_sound_neg_type.
+  Proof.
+    intros x pre.
+    funelim (_uconv x) ; cbn in pre |- *.
+
+    3: simp uconv_ne ; cbn ; destruct (build_ne_view2 _ _) eqn:e ; cbn ; try easy.
+    2: simp uconv_tm_red ; cbn ; destruct (build_nf_view2 _ _) eqn:e ; cbn ; try easy.
+    1: simp uconv_tm ; cbn.
+
+    all:
+      repeat (match goal with | H : ∑ _, _ |- _ => destruct H as [? pre] end) ;
+      repeat (match goal with | A : class |- _ => destruct A ; cbn in * end) ; try easy.
+    
+    - intros T' []%red_sound V' []%red_sound.
+      eapply typeConvRed_prem2 in pre ; tea.
+      unshelve eexists.
+      1: repeat eexists ; eauto using type_class_ty.
+      intros [|] _ Hnty ; cbn in * ; [easy|..].
+      intros Hty.
+      eapply Hnty.
+      etransitivity.
+      2: etransitivity ; tea.
+      1: symmetry. 
+      all: eapply RedConvTyC, subject_reduction_type ; eauto.
+      all: boundary.
+    
+    - intros ? []%red_sound ? []%red_sound.
+      eapply termConvRed_prem3 in pre ; tea.
+      2: reflexivity.
+      unshelve eexists.
+      1: repeat eexists ; eauto using term_class_ty.
+      intros [|] _ Hnty ; cbn in * ; [easy|..].
+      intros Hty.
+      eapply Hnty.
+      eapply TermConv ; refold.
+      2: constructor ; boundary.
+      etransitivity.
+      2: etransitivity ; [eassumption|..].
+      1: symmetry.
+      all: eapply RedConvTeC, subject_reduction ; [..|eassumption].
+      all: boundary.
+
+    - epose proof pre as [? ? [[]%typePiCongAlg_prem0]%dup].
+      unshelve eexists.
+      1: repeat eexists ; eauto using type_class_ty.
+      intros [|] Hty ? ; cbn in *.
+      2: now intros []%prod_ty_inj.
+      eapply implem_uconv_graph, uconv_sound_decl in Hty as [Hty _] ; cbn in Hty.
+      edestruct typePiCongAlg_prem1 ; eauto.
+      unshelve eexists.
+      1: repeat eexists ; eauto using type_class_ty.
+      intros [|] _ Hty' ; [easy|..].
+      intros []%prod_ty_inj.
+      eapply Hty', stability1 ; eauto.
+
+    - epose proof pre as [?? [[(?&[-> _ _]&?)%termGen' _]]%dup].
+      assert ([projT1 |-[ de ] tProd A B : U] × [projT1 |-[ de ] tProd A' B' : U]) as pre''.
+      {
+        split.
+        all: eapply ty_conv ; [eauto|..].
+        all: now symmetry.
+      }
+      edestruct termPiCongAlg_prem0 ; eauto.
+      unshelve eexists.
+      1: repeat eexists ; eauto using term_class_ty.
+      intros [|] Hty Hnty ; cbn in *.
+      2:{ 
+        intros ?.
+        eapply Hnty, prod_tm_inj.
+        econstructor ; now symmetry.
+      }
+      eapply implem_uconv_graph, uconv_sound_decl in Hty as [_ ?]; tea.
+      edestruct termPiCongAlg_prem1 ; eauto.
+      unshelve eexists.
+      1: repeat eexists ; eauto using term_class_ty.
+      intros [|] Hty Hnty' ; cbn in * ; [easy|..].
+      intros ?.
+      eapply Hnty', stability1.
+      1: now econstructor.
+      eapply prod_tm_inj.
+      now eapply convtm_conv ; [..|symmetry].
+
+    - epose proof pre as [? ? [[]%typeSigCongAlg_prem0]%dup].
+      unshelve eexists.
+      1: repeat eexists ; eauto using type_class_ty.
+      intros [|] Hty ? ; cbn in *.
+      2: now intros []%sig_ty_inj.
+      eapply implem_uconv_graph, uconv_sound_decl in Hty as [Hty _] ; cbn in Hty.
+      edestruct typeSigCongAlg_prem1 ; eauto.
+      unshelve eexists.
+      1: repeat eexists ; eauto using type_class_ty.
+      intros [|] _ Hty' ; [easy|..].
+      intros []%sig_ty_inj.
+      now eapply Hty'.
+
+    - epose proof pre as [?? [pre' [(?&[-> _ _]&?)%termGen' _]]%dup].
+      assert ([projT1 |-[ de ] tSig A B : U] × [projT1 |-[ de ] tSig A' B' : U]) as pre''.
+      {
+        split.
+        all: eapply ty_conv ; [eauto|..].
+        all: now symmetry.
+      }
+      edestruct termSigCongAlg_prem0 ; eauto.
+      unshelve eexists.
+      1: repeat eexists ; eauto using term_class_ty.
+      intros [|] Hty Hnty ; cbn in *.
+      2:{ 
+        intros ?.
+        eapply Hnty, sig_tm_inj.
+        now econstructor ; [..|symmetry].
+      }
+      eapply implem_uconv_graph, uconv_sound_decl in Hty as [_ ?]; tea.
+      edestruct termSigCongAlg_prem1 ; eauto.
+      unshelve eexists.
+      1: repeat eexists ; eauto using term_class_ty.
+      intros [|] Hty Hnty' ; cbn in * ; [easy|..].
+      intros ?.
+      eapply Hnty', sig_tm_inj.
+      now eapply convtm_conv ; [..|symmetry].
+    
+    - epose proof pre as [_ _ [pre' []%typeIdCongAlg_prem0]%dup].
+      unshelve eexists.
+      1: repeat eexists ; eauto using type_class_ty.
+      intros [|] Hty ? ; cbn.
+      2: now intros [? _]%id_ty_inj.
+      eapply implem_uconv_graph, uconv_sound_decl in Hty as [? _] ; eauto.
+      edestruct typeIdCongAlg_prem1 ; eauto.
+      unshelve eexists.
+      1: repeat eexists ; eauto using term_class_ty.
+      intros [|] Hty' ? ; cbn in *.
+      2: now intros []%id_ty_inj.
+      eapply implem_uconv_graph, uconv_sound_decl in Hty' ; tea.
+      edestruct typeIdCongAlg_prem2 ; eauto.
+      unshelve eexists.
+      1: repeat eexists ; eauto using term_class_ty.
+      intros [|] ? Hty'' ; cbn in * ; [easy|..].
+      now intros []%id_ty_inj.
+    
+    - epose proof pre as [?? [pre' [(?&[-> _ _]&?)%termGen' _]]%dup].
+      assert ([projT1 |-[ de ] tId A x y : U] × [projT1 |-[ de ] tId A' x' y' : U]) as pre''.
+      {
+        split.
+        all: eapply ty_conv ; [eauto|..].
+        all: now symmetry.
+      }
+      edestruct termIdCongAlg_prem0 ; eauto.
+      unshelve eexists.
+      1: repeat eexists ; eauto using term_class_ty.
+      intros [|] Hty Hnty ; cbn in *.
+      2: now eintros ?%convtm_conv%id_tm_inj ; [..|now symmetry] ; eauto.
+      eapply implem_uconv_graph, uconv_sound_decl in Hty ; eauto.
+      edestruct termIdCongAlg_prem1 ; eauto.
+      unshelve eexists.
+      1: repeat eexists ; eauto using term_class_ty.
+      intros [|] Hty'%implem_uconv_graph Hnty' ; cbn in *.
+      2: now eintros ?%convtm_conv%id_tm_inj ; [..|now symmetry] ; eauto.
+      eapply uconv_sound_decl in Hty' ; tea.
+      edestruct termIdCongAlg_prem2 ; eauto.
+      unshelve eexists.
+      1: repeat eexists ; eauto using term_class_ty, type_class_ty.
+      intros [|] ? Hty'' ; cbn in * ; [easy|..].
+      now eintros ?%convtm_conv%id_tm_inj ; [..|now symmetry] ; eauto.
+
+    - destruct pre as [wt wu [Ht Hu]].
+      eapply type_isType in Ht ; tea.
+      inversion Ht ; inversion H.
+
+    - edestruct LamCongUAlg_prem0 as (?&[]) ; eauto.
+      unshelve eexists.
+      1: repeat eexists ; eauto using term_class_ty.
+      intros [|] Hty Hnty ; cbn in * ; [easy|..].
+      eintros Hty'%convtm_conv ; [..|now symmetry].
+      eapply Hnty.
+      eapply convtm_red'.
+      3: reflexivity.
+      1,2: now eapply redalg_one_step, eta_expand_beta.
+      eapply convtm_meta_conv.
+      3: reflexivity.
+      2: shelve.
+      econstructor.
+      2: now do 2 econstructor ; [boundary|econstructor].
+      erewrite <- !wk1_ren_on.
+      erewrite wk_prod.
+      eapply typing_wk ; boundary.
+      Unshelve.
+      now bsimpl.
+      
+    - destruct pre as [wt wu [Ht Hu]].
+      eapply type_isType in Ht ; tea.
+      inversion Ht ; inversion H.
+
+    - edestruct LamNeUAlg_prem0 as (?&[]) ; eauto.
+      unshelve eexists.
+      1: repeat eexists ; eauto using term_class_ty.
+      intros [|] Hty Hnty ; cbn in * ; [easy|..].
+      eintros Hty'%convtm_conv ; [..|now symmetry].
+      eapply Hnty.
+      eapply convtm_red'.
+      3: reflexivity.
+      1: now eapply redalg_one_step, eta_expand_beta.
+      1: reflexivity.
+      eapply convtm_meta_conv.
+      3: reflexivity.
+      2: shelve.
+      econstructor.
+      2: now do 2 econstructor ; [boundary|econstructor].
+      erewrite <- !wk1_ren_on.
+      erewrite wk_prod.
+      eapply typing_wk ; boundary.
+      Unshelve.
+      now bsimpl.
+    
+    - destruct pre as [wt wu [Ht Hu]].
+      eapply type_isType in Hu ; tea.
+      inversion Hu ; inversion H.
+
+    - edestruct NeLamUAlg_prem0 as (?&[]) ; eauto.
+      unshelve eexists.
+      1: repeat eexists ; eauto using term_class_ty.
+      intros [|] Hty Hnty ; cbn in * ; [easy|..].
+      eintros Hty'%convtm_conv ; [..|now symmetry].
+      eapply Hnty.
+      eapply convtm_red'.
+      3: reflexivity.
+      2: now eapply redalg_one_step, eta_expand_beta.
+      1: reflexivity.
+      eapply convtm_meta_conv.
+      3: reflexivity.
+      2: shelve.
+      econstructor.
+      2: now do 2 econstructor ; [boundary|econstructor].
+      erewrite <- !wk1_ren_on.
+      erewrite wk_prod.
+      eapply typing_wk ; boundary.
+      Unshelve.
+      now bsimpl.
+
+    - destruct pre as [wt wu [Ht Hu]].
+      eapply type_isType in Hu ; tea.
+      inversion Hu ; inversion H.
+        
+    - epose proof pre as [?? [pre' [(?&[->]&?)%termGen']]%dup].
+      edestruct termSuccCongAlg_prem0.
+      1: split ; eapply ty_conv ; eauto ; now symmetry.
+      unshelve eexists.
+      1: repeat eexists ; eauto using term_class_ty.
+      intros [|] ? Hty ; cbn in * ; [easy|..].
+      eintros Hconv%convtm_conv ; [..|now symmetry].
+      unshelve eapply nat_conv_inj in Hconv.
+      1-2: now constructor.
+      now cbn in Hconv.
+
+    - destruct pre as [wt wu [Ht Hu]].
+      epose proof Ht as Ht'%type_isType ; tea.
+      inversion Ht' ; inversion H.
+
+    - edestruct PairCongUAlg_prem0 as [] ; eauto.
+      unshelve eexists.
+      1: repeat eexists ; eauto using term_class_ty.
+      intros [|] Hty Hnty ; cbn in *.
+      2: now eintros ?%pair_conv_fst.
+      eapply implem_uconv_graph, uconv_sound_decl in Hty as [_ ?].
+      edestruct PairCongUAlg_prem1 ; eauto.
+      unshelve eexists.
+      1: repeat eexists ; eauto using term_class_ty.
+      intros [|] Hty Hnty' ; cbn in * ; [easy|..].
+      now eintros ?%pair_conv_snd.
+
+    - destruct pre as [wt wu [Ht Hu]].
+      epose proof Ht as Ht'%type_isType ; tea.
+      inversion Ht' ; inversion H.
+
+    - edestruct PairNeUAlg_prem0 as [] ; eauto.
+      unshelve eexists.
+      1: repeat eexists ; eauto using term_class_ty.
+      intros [|] Hty Hnty ; cbn in *.
+      2: now eintros ?%pair_conv_fst_ne.
+      eapply implem_uconv_graph, uconv_sound_decl in Hty as [_ ?].
+      edestruct PairNeUAlg_prem1 ; eauto.
+      unshelve eexists.
+      1: repeat eexists ; eauto using term_class_ty.
+      intros [|] Hty Hnty' ; cbn in * ; [easy|..].
+      now eintros ?%pair_conv_snd_ne.
+      
+    - destruct pre as [wt wu [Ht Hu]].
+      epose proof Hu as Hu'%type_isType ; tea.
+      inversion Hu' ; inversion H.
+
+    - edestruct NePairUAlg_prem0 as [] ; eauto.
+      unshelve eexists.
+      1: repeat eexists ; eauto using term_class_ty.
+      intros [|] Hty Hnty ; cbn in *.
+      2: now eintros ?%pair_conv_ne_fst.
+      eapply implem_uconv_graph, uconv_sound_decl in Hty as [_ ?].
+      edestruct NePairUAlg_prem1 ; eauto.
+      unshelve eexists.
+      1: repeat eexists ; eauto using term_class_ty.
+      intros [|] Hty Hnty' ; cbn in * ; [easy|..].
+      now eintros ?%pair_conv_ne_snd.
+
+    - destruct pre as [? ? ?].
+      eapply nf_view2_neutral_can in e as [wt%not_can_whne wu%not_can_whne] ; tea.
+      edestruct typeNeuConvAlg_prem2 ; cycle 2 ; tea.
+      unshelve eexists.
+      1: eexists ; now split.
+      intros [|] _ Hnty ; cbn in * ; [easy|..].
+      unshelve eintros ?%ty_conv_inj.
+      1-2: now constructor.
+      cbn in *.
+      eauto.
+      eapply Hnty.
+      eexists.
+      now eapply conv_neu_conv.
+
+    - destruct pre as [? ? ?].
+      eapply nf_view2_neutral_can in e as [wt%not_can_whne wu%not_can_whne] ; tea.
+      unshelve eexists.
+      1: now repeat eexists.
+      cbn in *.
+      intros [|] _ Hnty ; cbn in * ; eauto.
+      intros ?.
+      eapply Hnty.
+      eexists.
+      now eapply conv_neu_conv.
+
+    - destruct pre as [wt wu [Ht Hu]].
+      eapply type_isType in Ht, Hu ; tea.
+      unshelve eintros H_view%ty_conv_inj ; tea.
+      eapply mismatch2_hd_view_ty in e.
+      now erewrite e in H_view.
+
+    - intros Hty.
+      assert (whne t -> whne u -> False) by
+       (now intros ; eapply mismatch2_hd_view_ne ; cycle -1).
+      eapply mismatch2_hd_view_tm in e as [e|[e|e]] ; eauto.
+      + destruct e as (nft&nfu&e).
+        enough (type_hd_view _ nft nfu) as Hhd by now rewrite e in Hhd.
+        apply ty_conv_inj.
+        econstructor.
+        econstructor ; tea.
+        destruct nft.
+        all: try solve [eapply boundary_tm_conv_l in Hty as (?&Hgen&?)%termGen' ;
+          cbn in Hgen ; try easy ; prod_hyp_splitter ; subst ; try solve [now symmetry]].
+        destruct nfu ; [..|easy].
+        all: solve [eapply boundary_tm_conv_r in Hty as (?&Hgen&?)%termGen' ;
+          cbn in Hgen ; try easy ; prod_hyp_splitter ; subst ; try solve [now symmetry]].
+      + destruct e as (nft&nfu&e).
+        enough (nat_hd_view _ nft nfu) as Hhd by now rewrite e in Hhd.
+        apply nat_conv_inj.
+        econstructor ; tea.
+        destruct nft.
+        all: try solve [eapply boundary_tm_conv_l in Hty as (?&Hgen&?)%termGen' ;
+          cbn in Hgen ; try easy ; prod_hyp_splitter ; subst ; try solve [now symmetry]].
+        destruct nfu ; [..|easy].
+        all: solve [eapply boundary_tm_conv_r in Hty as (?&Hgen&?)%termGen' ;
+          cbn in Hgen ; try easy ; prod_hyp_splitter ; subst ; try solve [now symmetry]].
+
+      + destruct e as (nft&nfu&e).
+        enough (∑ Γ A x y, id_hd_view Γ A x y nft nfu) as (?&?&?&?&?Hhd)
+          by now rewrite e in Hhd.
+        destruct nft.
+        * epose proof Hty as (?&Hgen&?)%boundary_tm_conv_l%termGen' ;
+          cbn in Hgen ; try easy ; prod_hyp_splitter ; subst.
+          do 4 eexists.
+          eapply id_conv_inj.
+          econstructor ; tea.
+          now symmetry.
+        * destruct nfu ; [..|easy].
+          epose proof Hty as (?&Hgen&?)%boundary_tm_conv_r%termGen' ;
+          cbn in Hgen ; try easy ; prod_hyp_splitter ; subst.
+          do 4 eexists.
+          eapply id_conv_inj.
+          econstructor ; tea.
+          now symmetry.
+
+    - destruct (Nat.eqb_spec n n') ; cbn ; try easy.
+      intros [? (?&[[= ->]])%neuConvGen].
+      eauto.
+
+    - edestruct neuAppCongAlg_prem0 ; eauto.
+      destruct pre as [wn wn' []].
+      inversion wn ; inversion wn' ; subst.
+      unshelve eexists.
+      1: eexists ; now split.
+      intros [|] Hty%implem_uconv_graph Hnty ; cbn in *.
+      2: now intros [? (?&?&?&?&[[=]])%neuConvGen] ; subst.
+      eapply uconv_sound_decl in Hty as [? Hty] ; eauto.
+      eapply AppCongUAlg_bridge in Hty as (?&?&[? Hty]) ; eauto.
+      edestruct neuAppCongAlg_prem1 ; eauto.
+      unshelve eexists.
+      1: repeat eexists ; eauto using term_class_ty.
+      intros  [|] _ Hnty' ; [easy|..].
+      intros [? (?&?&?&?&[[=]])%neuConvGen] ; subst.
+      eapply Hnty'.
+      econstructor ; tea.
+      eapply prod_ty_inj, Hty.
+      boundary.
+
+    - edestruct neuNatElimCong_prem0 ; eauto.
+      destruct pre as [wn wn' []].
+      inversion wn ; inversion wn' ; subst.
+      unshelve eexists.
+      1: eexists ; now split.
+      intros [|] Hty%implem_uconv_graph Hnty ; cbn in *.
+      2: now intros [? (?&?&?&?&[[=]])%neuConvGen] ; subst.
+      eapply uconv_sound_decl in Hty as [? Hty] ; eauto.
+      eapply NatElimCongUAlg_bridge in Hty as [? Hty] ; eauto.
+      edestruct neuNatElimCong_prem1 ; eauto.
+      unshelve eexists.
+      1: repeat eexists ; eauto using type_class_ty.
+      intros  [|] HP%implem_uconv_graph Hnty' ; cbn.
+      2: now intros [? (?&?&?&?&[[=]])%neuConvGen] ; subst.
+      eapply uconv_sound_decl in HP as [? _].
+      edestruct neuNatElimCong_prem2 ; eauto.
+      unshelve eexists.
+      1: repeat eexists ; eauto using term_class_ty.
+      intros  [|] Hz%implem_uconv_graph ? ; cbn.
+      2: now intros [? (?&?&?&?&[[=]])%neuConvGen] ; subst.
+      eapply uconv_sound_decl in Hz as [_ ?].
+      edestruct neuNatElimCong_prem3 ; eauto.
+      unshelve eexists.
+      1: repeat eexists ; eauto using term_class_ty.
+      intros  [|] Hs%implem_uconv_graph ? ; cbn ; [easy|..].
+      now intros [? (?&?&?&?&[[=]])%neuConvGen] ; subst.
+
+    - edestruct neuEmptyElimCong_prem0 ; eauto.
+      destruct pre as [wn wn' []].
+      inversion wn ; inversion wn' ; subst.
+      unshelve eexists.
+      1: eexists ; now split.
+      intros [|] Hty%implem_uconv_graph Hnty ; cbn in *.
+      2: now intros [? (?&?&[[=]])%neuConvGen] ; subst.
+      eapply uconv_sound_decl in Hty as [? Hty] ; eauto.
+      eapply EmptyElimCongUAlg_bridge in Hty as [? Hty] ; eauto.
+      edestruct neuEmptyElimCong_prem1 ; eauto.
+      unshelve eexists.
+      1: repeat eexists ; eauto using type_class_ty.
+      intros  [|] HP%implem_uconv_graph Hnty' ; cbn ; [easy|..].
+      now intros [? (?&?&[[=]])%neuConvGen] ; subst.
+
+    - edestruct neuFstCongAlg_prem0 ; eauto.
+      destruct pre as [wn wn' []].
+      inversion wn ; inversion wn' ; subst.
+      unshelve eexists.
+      1: eexists ; now split.
+      intros [|] Hty%implem_uconv_graph Hnty ; cbn in * ; [easy|..].
+      now intros [? (?&?&?&[[=]])%neuConvGen] ; subst.
+
+    - edestruct neuSndCongAlg_prem0 ; eauto.
+      destruct pre as [wn wn' []].
+      inversion wn ; inversion wn' ; subst.
+      unshelve eexists.
+      1: eexists ; now split.
+      intros [|] Hty%implem_uconv_graph Hnty ; cbn in * ; [easy|..].
+      now intros [? (?&?&?&[[=]])%neuConvGen] ; subst.
+
+    - edestruct neuIdElimCong_prem0 ; eauto.
+      destruct pre as [wn wn' []].
+      inversion wn ; inversion wn' ; subst.
+      unshelve eexists.
+      1: eexists ; now split.
+      intros [|] Hty%implem_uconv_graph Hnty ; cbn in *.
+      2: now intros [? (?&?&?&?&?&?&[[=]])%neuConvGen] ; subst.
+      eapply uconv_sound_decl in Hty as [? Hty] ; eauto.
+      eapply IdElimCongUAlg_bridge in Hty as (?&?&?&[? Hty]) ; eauto.
+      edestruct neuIdElimCong_prem1 ; eauto.
+      unshelve eexists.
+      1: repeat eexists ; eauto using type_class_ty.
+      intros  [|] HP%implem_uconv_graph Hnty' ; cbn.
+      2: now intros [? (?&?&?&?&?&?&[[=]])%neuConvGen] ; subst.
+      eapply uconv_sound_decl in HP as [? _].
+      edestruct neuIdElimCong_prem2 ; eauto.
+      unshelve eexists.
+      1: repeat eexists ; eauto using term_class_ty.
+      intros  [|] Hz%implem_uconv_graph ? ; cbn ; [easy|..].
+      now intros [? (?&?&?&?&?&?&[[=]])%neuConvGen] ; subst.
+
+    - intros [? ?%neuConvGen].
+      destruct t ; cbn in * ; try solve [easy].
+      all: prod_hyp_splitter ; subst.
+      all: simp build_ne_view2 in e ; cbn in *.
+      all: congruence.
+    
+  Qed.
+
+  Corollary implem_tconv_sound_neg Γ T V e :
+    graph tconv (Γ,T,V) (exception e) ->
+    [Γ |-[de] T] -> [Γ |-[de] V] ->
+    ~ [Γ |-[de] T ≅ V].
+  Proof.
+    intros Hgraph **.
+    eapply (funrect_graph _
+      (fun '(Γ',T',V') => [Γ' |-[de] T'] × [Γ' |-[de] V'])
+      (fun '(Γ',T',V') r => match r with | success _ => True | exception _ => ~ [Γ' |-[de] T' ≅ V'] end)) in Hgraph ; try easy.
+    
+    intros (?&?&?) [].
+    funelim (tconv _) ; cbn.
+    inversion_clear eqargs.
+    intros [] ; cbn ; [easy|].
+    eintros ?%funrect_graph.
+    2: now apply _implem_conv_neg_sound.
+    all: now cbn in *.
+  Qed.
+
+End ConvSoundNeg.
