theories/Decidability/Views.v
@@ -1,0 +1,295 @@
+(** * LogRel.Decidability.Views: properties of the view-building functions. *)
+From Coq Require Import Nat Lia.
+From Equations Require Import Equations.
+From PartialFun Require Import Monad PartialFun MonadExn.
+From LogRel Require Import Utils BasicAst AutoSubst.Extra Context NormalForms Notations PropertiesDefinition DeclarativeTyping NeutralConvProperties.
+From LogRel.Decidability Require Import Functions UntypedFunctions.
+
+Import MonadNotations.
+Set Universe Polymorphism.
+Set Polymorphic Inductive Cumulativity.
+Set Printing Universes.
+
+Import DeclarativeTypingProperties.
+
+Lemma zip_can t s : ~ isCanonical (zip1 t s).
+Proof.
+  destruct s ; cbn.
+  all: now intros c ; inversion c.
+Qed.
+
+Lemma isType_tm_view1 t e :
+  build_tm_view1 t = tm_view1_type e ->
+  isType t × ~ whne t.
+Proof.
+  intros H.
+  destruct e ; cbn.
+  all: split ; [ now econstructor | intros H' ; inversion H'].
+Qed.
+
+Lemma whnf_tm_view1_nat t e :
+  build_tm_view1 t = tm_view1_nat e ->
+  whnf t × ~ whne t.
+Proof.
+  intros H.
+  destruct e ; cbn.
+  all: split ; [ now econstructor | intros H' ; inversion H'].
+Qed.
+
+
+Lemma ty_view1_small_can T n : build_ty_view1 T = ty_view1_small n -> ~ isCanonical T.
+Proof.
+  destruct T ; cbn.
+  all: inversion 1.
+  all: inversion 1.
+Qed.
+
+Lemma tm_view1_neutral_can t n : build_nf_view1 t = nf_view1_ne n -> ~ isCanonical t.
+Proof.
+  destruct t ; cbn.
+  all: inversion 1.
+  all: inversion 1.
+Qed.
+
+Lemma ty_view2_neutral_can T V : build_nf_ty_view2 T V = ty_neutrals T V -> ~ isCanonical T × ~ isCanonical V.
+Proof.
+  destruct T, V ; cbn.
+  all: inversion 1.
+  all: split ; inversion 1.
+Qed.
+
+
+Lemma whnf_view3_ty_neutral_can s t u : build_nf_view3 (tSort s) t u = types s (ty_neutrals t u) -> ~ isCanonical t × ~ isCanonical u.
+Proof.
+  destruct t, u ; cbn.
+  all: inversion 1.
+  all: split ; inversion 1.
+Qed.
+
+Lemma whnf_view3_neutrals_can A t u :
+  whnf A ->
+  build_nf_view3 A t u = neutrals A t u ->
+  [× isPosType A, ~ isCanonical t & ~ isCanonical u].
+Proof.
+  intros HA.
+  simp build_nf_view3.
+  destruct (build_ty_view1 A) eqn:EA ; cbn.
+  all: try solve [inversion 1].
+  1: match goal with | |- context [match ?t with | _ => _ end] => destruct t eqn:? ; cbn end ;
+    try solve [inversion 1].
+  all: simp build_nf_view3 ; cbn.
+  all: destruct (build_nf_view1 t) eqn:? ; cbn.
+  all: try solve [inversion 1].
+  all: repeat (
+    match goal with | |- context [match ?t with | _ => _ end] => destruct t eqn:? ; cbn end ;
+    try solve [inversion 1]).
+  all: intros _.
+  all: split ; try solve [now eapply tm_view1_neutral_can].
+  all: econstructor.
+  eapply ty_view1_small_can in EA.
+  destruct HA ; try easy.
+  all: exfalso ; apply EA ; now constructor.
+Qed.
+
+Definition whne_ne_view1 {N} (w : whne N) : ne_view1 N :=
+  match w with
+  | whne_tRel => ne_view1_rel _
+  | whne_tApp _ => ne_view1_dest _ (eApp _)
+  | whne_tNatElim _ => ne_view1_dest _ (eNatElim _ _ _)
+  | whne_tEmptyElim _ => ne_view1_dest _ (eEmptyElim _)
+  | whne_tFst _ => ne_view1_dest _ eFst
+  | whne_tSnd _ => ne_view1_dest _ eSnd
+  | whne_tIdElim _ => ne_view1_dest _ (eIdElim _ _ _ _ _)
+  end.
+
+Lemma whne_ty_view1 {N} (w : whne N) : build_ty_view1 N = ty_view1_small (whne_ne_view1 w).
+Proof.
+  now destruct w.
+Qed.
+
+Lemma whne_nf_view1 {N} (w : whne N) : build_nf_view1 N = nf_view1_ne (whne_ne_view1 w).
+Proof.
+  now destruct w.
+Qed.
+
+Lemma whne_ty_view2 {M N} (wM : whne M) (wN : whne N) : build_nf_ty_view2 M N = ty_neutrals M N.
+Proof.
+  simp build_nf_ty_view2.
+  unshelve erewrite ! whne_ty_view1 ; tea.
+  now reflexivity.
+Qed.
+
+Lemma whne_nf_view3 P m n (wP : isPosType P) (wm : whne m) (wn : whne n) :
+  build_nf_view3 P m n =
+    (match wP with
+    | UnivPos => types _ (ty_neutrals m n)
+    | _ => neutrals _ m n
+    end).
+Proof.
+  simp build_nf_view3.
+  destruct wP ; cbn.
+  2-4: unshelve erewrite whne_nf_view1 ; tea; cbn; now rewrite (whne_nf_view1 wn).
+  - rewrite whne_ty_view2 ; cbn ; tea.
+    reflexivity.
+  - unshelve erewrite whne_ty_view1 ; tea.
+    cbn.
+    unshelve erewrite whne_nf_view1 ; tea ; cbn.
+    destruct (build_nf_view1 _) eqn:e ; try easy.
+    all: unshelve erewrite whne_nf_view1 in e ; tea.
+    all: inversion e.
+Qed.
+
+Lemma ty_mismatch_hd_view Γ T V (tT : isType T) (tV : isType V) :
+  build_nf_ty_view2 T V = ty_mismatch T V ->
+  type_hd_view Γ tT tV = False.
+Proof.
+  destruct tT, tV ; cbn ; try reflexivity.
+  all: simp build_nf_ty_view2 ; cbn.
+  1-6: congruence.
+  do 2 (unshelve erewrite whne_ty_view1 ; tea) ; cbn.
+  congruence.
+Qed.
+
+Lemma univ_mismatch_hd_view Γ s T V (tT : isType T) (tV : isType V) :
+  build_nf_view3 (tSort s) T V = types s (ty_mismatch T V) ->
+  univ_hd_view Γ tT tV = False.
+Proof.
+  destruct tT, tV ; cbn ; try reflexivity.
+  all: simp build_nf_view3 build_nf_ty_view2 ; cbn.
+  1-5: intros [=].
+  do 2 (unshelve erewrite whne_ty_view1 ; tea) ; cbn.
+  discriminate.
+Qed.
+
+Lemma mismatch_hd_view Γ A t u (tA : isType A) :
+  whnf t -> whnf u ->
+  build_nf_view3 A t u = mismatch A t u ->
+  (∑ (nft : isNat t) (nfu : isNat u), A = tNat × nat_hd_view Γ nft nfu = False) +
+  (∑ (nft : isId t) (nfu : isId u) A' x y, A = tId A' x y × id_hd_view Γ A' x y nft nfu = False).
+Proof.
+  intros wt wu.
+  destruct tA ; cbn.
+  all: simp build_nf_view3 build_nf_ty_view2 ; cbn.
+  all: try solve [intros [=]].
+  - destruct (build_nf_view1 t), (build_nf_view1 u) ; cbn.
+    all: try solve [intros [=]].
+    all: destruct n ; cbn ; try solve [intros [=]].
+    all: destruct n0 ; cbn ; try solve [intros [=]].
+    all: unshelve (intros _ ; left ; do 2 eexists).
+    all: try solve [constructor].
+    1-8: econstructor ; eapply not_can_whne ; tea ; solve [now apply zip_can | intros c ; inversion c].
+    all: now cbn.
+
+  - destruct (build_nf_view1 t), (build_nf_view1 u) ; cbn.
+    all: solve [intros [=]].
+
+  - destruct (build_nf_view1 t), (build_nf_view1 u) ; cbn.
+    all: try solve [intros [=]]. 
+    all: destruct n ; cbn ; try solve [intros [=]].
+    all: (intros _ ; right ; do 5 eexists).
+    all: split ; [reflexivity|..].
+    Unshelve.
+    all: try solve [constructor].
+    5-8: econstructor ; eapply not_can_whne ; tea ; solve [now apply zip_can | intros c ; inversion c].
+    all: now cbn.
+    
+  - unshelve erewrite whne_ty_view1 ; tea ; cbn.
+    destruct (build_nf_view1 t) ; cbn ; try solve [intros [=]].
+    destruct (build_nf_view1 u) ; cbn ; solve [intros [=]].
+
+Qed.
+
+Definition ncan_ne_view1 {N} (w : ~ isCanonical N) : ne_view1 N.
+Proof.
+  destruct N.
+  all: try solve [destruct w ; econstructor].
+  - now constructor.
+  - eapply (ne_view1_dest _ (eApp _)).
+  - eapply (ne_view1_dest _ (eNatElim _ _ _)).
+  - eapply (ne_view1_dest _ (eEmptyElim _)).
+  - eapply (ne_view1_dest _ eFst).
+  - eapply (ne_view1_dest _ eSnd).
+  - eapply (ne_view1_dest _ (eIdElim _ _ _ _ _)).
+Defined.
+
+
+Lemma ncan_nf_view1 {N} (w : ~ isCanonical N) :
+  build_nf_view1 N = nf_view1_ne (ncan_ne_view1 w).
+Proof.
+  destruct N ; cbn ; try reflexivity.
+  all: destruct w ; econstructor.
+Qed.
+
+Lemma nf_view2_neutral_can t t' :
+  build_nf_view2 t t' = neutrals2 t t' ->
+  ~ isCanonical t /\ ~ isCanonical t'.
+Proof.
+  intros Heq.
+  simp build_nf_view2 in Heq.
+  destruct (build_nf_view1 t) as [? [] | | ? [] | | | ] eqn:Heqt ; cbn in Heq.
+  all: destruct (build_nf_view1 t') as [? [] | | ? [] | | | ] eqn:Heqt' ; cbn in Heq.
+  all: try solve [congruence].
+  split.
+  all: now eapply tm_view1_neutral_can.
+Qed.
+
+Definition nf_view2_rename (ρ : nat -> nat) {t t' : term} (v : nf_view2 t t') : nf_view2 t⟨ρ⟩ t'⟨ρ⟩ :=
+  match v in nf_view2 x x' return nf_view2 x⟨ρ⟩ x'⟨ρ⟩ with
+  | sorts2 s s' => sorts2 s s'
+  | prods2 A A' B B' => prods2 A⟨ρ⟩ A'⟨ρ⟩ B⟨upRen_term_term ρ⟩ B'⟨upRen_term_term ρ⟩
+  | nats2 => nats2
+  | emptys2 => emptys2
+  | sigs2 A A' B B' => sigs2 A⟨ρ⟩ A'⟨ρ⟩ B⟨upRen_term_term ρ⟩ B'⟨upRen_term_term ρ⟩
+  | ids2 A A' x x' y y' => ids2 A⟨ρ⟩ A'⟨ρ⟩ x⟨ρ⟩ x'⟨ρ⟩ y⟨ρ⟩ y'⟨ρ⟩
+  | lams2 A A' t t' => lams2 A⟨ρ⟩ A'⟨ρ⟩ t⟨upRen_term_term ρ⟩ t'⟨upRen_term_term ρ⟩
+  | lam_ne2 A t n' => lam_ne2 A⟨ρ⟩ t⟨upRen_term_term ρ⟩ n'⟨ρ⟩
+  | ne_lam2 n A' t' => ne_lam2 n⟨ρ⟩ A'⟨ρ⟩ t'⟨upRen_term_term ρ⟩
+  | zeros2 => zeros2
+  | succs2 t t' => succs2 t⟨ρ⟩ t'⟨ρ⟩
+  | pairs2 A A' B B' t t' u u' =>
+      pairs2 A⟨ρ⟩ A'⟨ρ⟩ B⟨upRen_term_term ρ⟩ B'⟨upRen_term_term ρ⟩ t⟨ρ⟩ t'⟨ρ⟩ u⟨ρ⟩ u'⟨ρ⟩
+  | pair_ne2 A B t u n' => pair_ne2 A⟨ρ⟩ B⟨upRen_term_term ρ⟩ t⟨ρ⟩ u⟨ρ⟩ n'⟨ρ⟩
+  | ne_pair2 n A' B' t' u' => ne_pair2 n⟨ρ⟩ A'⟨ρ⟩ B'⟨upRen_term_term ρ⟩ t'⟨ρ⟩ u'⟨ρ⟩
+  | refls2 A A' x x' => refls2 A⟨ρ⟩ A'⟨ρ⟩ x⟨ρ⟩ x'⟨ρ⟩
+  | neutrals2 n n' => neutrals2 n⟨ρ⟩ n'⟨ρ⟩
+  | mismatch2 t u => mismatch2 t⟨ρ⟩ u⟨ρ⟩
+  | anomaly2 t u => anomaly2 t⟨ρ⟩ u⟨ρ⟩
+  end.
+
+Lemma build_nf_view2_rename ρ t t' : build_nf_view2 t⟨ρ⟩ t'⟨ρ⟩ = nf_view2_rename ρ (build_nf_view2 t t').
+Proof.
+  destruct t, t' ; reflexivity.
+Qed.
+
+Definition ne_view2_rename (ρ : nat -> nat) {t t' : term} (v : ne_view2 t t') : ne_view2 t⟨ρ⟩ t'⟨ρ⟩ :=
+  match v in ne_view2 x x' return ne_view2 x⟨ρ⟩ x'⟨ρ⟩ with
+  | ne_rels n n' => ne_rels (ρ n) (ρ n')
+  | ne_apps f u f' u' => ne_apps f⟨ρ⟩ u⟨ρ⟩ f'⟨ρ⟩ u'⟨ρ⟩
+  | ne_nats n P hz hs n' P' hz' hs' => ne_nats
+      n⟨ρ⟩ P⟨upRen_term_term ρ⟩ hz⟨ρ⟩ hs⟨ρ⟩
+      n'⟨ρ⟩ P'⟨upRen_term_term ρ⟩ hz'⟨ρ⟩ hs'⟨ρ⟩
+  | ne_emptys n P n' P' => ne_emptys n⟨ρ⟩ P⟨upRen_term_term ρ⟩ n'⟨ρ⟩ P'⟨upRen_term_term ρ⟩
+  | ne_fsts p p' => ne_fsts p⟨ρ⟩ p'⟨ρ⟩
+  | ne_snds p p' => ne_snds p⟨ρ⟩ p'⟨ρ⟩
+  | ne_ids A x P hr y e A' x' P' hr' y' e' => ne_ids
+    A⟨ρ⟩ x⟨ρ⟩ P⟨upRen_term_term (upRen_term_term ρ)⟩ hr⟨ρ⟩ y⟨ρ⟩ e⟨ρ⟩
+    A'⟨ρ⟩ x'⟨ρ⟩ P'⟨upRen_term_term (upRen_term_term ρ)⟩ hr'⟨ρ⟩ y'⟨ρ⟩ e'⟨ρ⟩
+  | ne_mismatch t u => ne_mismatch t⟨ρ⟩ u⟨ρ⟩
+  | ne_anomaly t u => ne_anomaly t⟨ρ⟩ u⟨ρ⟩
+  end.
+
+Lemma build_ne_view2_rename ρ t t' : build_ne_view2 t⟨ρ⟩ t'⟨ρ⟩ = ne_view2_rename ρ (build_ne_view2 t t').
+Proof.
+  destruct t, t' ; reflexivity.
+Qed.
+
+Lemma mismatch2_hd_view_ty Γ T V (tT : isType T) (tV : isType V) :
+  build_nf_view2 T V = mismatch2 T V ->
+  type_hd_view Γ tT tV = False.
+Proof.
+  destruct tT, tV ; cbn ; try reflexivity.
+  all: simp build_nf_view2 ; cbn.
+  1-6: congruence.
+  do 2 (unshelve erewrite whne_nf_view1 ; tea ; cbn).
+  congruence.
+Qed.
